code/k256/Hacl.Impl.K256.PointDouble.fst
@@ -19,51 +19,52 @@ open Hacl.Impl.K256.Point
 
 
 inline_for_extraction noextract
-val point_double_no_alloc (out p:point) (tmp:lbuffer uint64 (4ul *! nlimb)) : Stack unit
+val point_double_no_alloc (out p:point) (tmp:lbuffer uint64 (5ul *! nlimb)) : Stack unit
   (requires fun h ->
     live h out /\ live h p /\ live h tmp /\
-    disjoint out p /\ disjoint out tmp /\ disjoint p tmp /\
+    eq_or_disjoint out p /\ disjoint out tmp /\ disjoint p tmp /\
     point_inv h p)
   (ensures fun h0 _ h1 -> modifies (loc out |+| loc tmp) h0 h1 /\ point_inv h1 out /\
     point_as_nat3_proj h1 out == S.point_double (point_as_nat3_proj h0 p))
 
 let point_double_no_alloc out p tmp =
-  let x, y, z = getx p, gety p, getz p in
+  let x1, y1, z1 = getx p, gety p, getz p in
   let x3, y3, z3 = getx out, gety out, getz out in
 
   let yy = sub tmp 0ul nlimb in
   let zz = sub tmp nlimb nlimb in
   let bzz3 = sub tmp (2ul *! nlimb) nlimb in
   let bzz9 = sub tmp (3ul *! nlimb) nlimb in
+  let tmp = sub tmp (4ul *! nlimb) nlimb in
 
-  fsqr yy y; //yy = y*y
-  fsqr zz z; //zz = z*z
+  fsqr yy y1; //yy = y*y
+  fsqr zz z1; //zz = z*z
 
-  fmul_small_num x3 x (u64 2); //x3 = 2*x
-  fmul x3 x3 y; //x3 = xy2 = x3*y = (2*x)*y
+  fmul_small_num x3 x1 (u64 2); //x3 = 2*x
+  fmul x3 x3 y1; //x3 = xy2 = x3*y = (2*x)*y
+
+  fmul tmp yy y1; //tmp = yy*y
+  fmul z3 tmp z1; //z3 = tmp*z = yy*y*z
+  fmul_small_num z3 z3 (u64 8); //z3 = z3*8=yy*y*z*8
 
   fmul_3b bzz3 zz; //bzz3 = (3*b)*zz
   fmul_small_num bzz9 bzz3 (u64 3); //bzz9 = 3*bzz3
 
   fsub bzz9 yy bzz9; //bzz9 = yy_m_bzz9 = yy-bzz9
-  fadd z3 yy bzz3; //z3 = yy_p_bzz3 = yy+bzz3
+  fadd tmp yy bzz3; //tmp = yy_p_bzz3 = yy+bzz3
 
   fmul y3 yy zz; //y3 = yy_zz = yy*zz
   fmul_24b y3 y3; //y3 = t = (24*b)*y3 = (24*b)*yy_zz
 
   fmul x3 x3 bzz9; //x3 = x3*bzz9 = xy2*yy_m_bzz9
 
-  fmul z3 bzz9 z3; //z3 = bzz9*z3 = yy_m_bzz9*yy_p_bzz3
-  fadd y3 z3 y3;  //y3 = z3+y3 = yy_m_bzz9*yy_p_bzz3+t
-
-  fmul z3 yy y; //z3 = yy*y
-  fmul z3 z3 z; //z3 = z3*z = yy*y*z
-  fmul_small_num z3 z3 (u64 8) //z3 = z3*8=yy*y*z*8
+  fmul tmp bzz9 tmp; //tmp = bzz9*tmp = yy_m_bzz9*yy_p_bzz3
+  fadd y3 tmp y3  //y3 = tmp+y3 = yy_m_bzz9*yy_p_bzz3+t
 
 
 val point_double (out p:point) : Stack unit
   (requires fun h ->
-    live h out /\ live h p /\ disjoint out p /\
+    live h out /\ live h p /\ eq_or_disjoint out p /\
     point_inv h p)
   (ensures fun h0 _ h1 -> modifies (loc out) h0 h1 /\ point_inv h1 out /\
     point_as_nat3_proj h1 out == S.point_double (point_as_nat3_proj h0 p))
@@ -71,6 +72,6 @@ val point_double (out p:point) : Stack unit
 [@CInline]
 let point_double out p =
   push_frame ();
-  let tmp = create (4ul *! nlimb) (u64 0) in
+  let tmp = create (5ul *! nlimb) (u64 0) in
   point_double_no_alloc out p tmp;
   pop_frame ()
