code/k256/Hacl.Impl.K256.PointMul.fst
@@ -1,0 +1,224 @@
+module Hacl.Impl.K256.PointMul
+
+open FStar.HyperStack
+open FStar.HyperStack.ST
+open FStar.Mul
+
+open Lib.IntTypes
+open Lib.Buffer
+
+module ST = FStar.HyperStack.ST
+module LSeq = Lib.Sequence
+module BSeq = Lib.ByteSequence
+
+module LE = Lib.Exponentiation
+module SE = Spec.Exponentiation
+module BE = Hacl.Impl.Exponentiation
+module ME = Hacl.Impl.MultiExponentiation
+
+module BD = Hacl.Bignum.Definitions
+module SD = Hacl.Spec.Bignum.Definitions
+module BC = Hacl.Bignum.Convert
+module SC = Hacl.Spec.Bignum.Convert
+
+module S = Spec.K256
+
+open Hacl.K256.Field
+open Hacl.Impl.K256.Point
+
+#set-options "--z3rlimit 50 --fuel 0 --ifuel 0"
+
+///////////////////////////////////////////
+
+unfold
+let linv_ctx (a:LSeq.lseq uint64 0) : Type0 = True
+
+unfold
+let refl (p:LSeq.lseq uint64 12{point_inv_lseq p}) : GTot S.aff_point =
+  S.to_aff_point (point_as_nat3_proj_lseq p)
+
+inline_for_extraction noextract
+let mk_to_k256_cm : BE.to_comm_monoid U64 12ul 0ul = {
+  BE.a_spec = S.aff_point;
+  BE.comm_monoid = S.mk_k256_cm;
+  BE.linv_ctx = linv_ctx;
+  BE.linv = point_inv_lseq;
+  BE.refl = refl;
+  }
+
+
+inline_for_extraction noextract
+val point_add : BE.lmul_st U64 12ul 0ul mk_to_k256_cm
+let point_add ctx x y xy =
+  let h0 = ST.get () in
+  S.to_aff_point_add_lemma (point_as_nat3_proj h0 x) (point_as_nat3_proj h0 y);
+  Hacl.Impl.K256.PointAdd.point_add xy x y
+
+
+inline_for_extraction noextract
+val point_double : BE.lsqr_st U64 12ul 0ul mk_to_k256_cm
+let point_double ctx x xx =
+  let h0 = ST.get () in
+  S.to_aff_point_double_lemma (point_as_nat3_proj h0 x);
+  Hacl.Impl.K256.PointDouble.point_double xx x
+
+
+inline_for_extraction noextract
+let mk_k256_concrete_ops : BE.concrete_ops U64 12ul 0ul = {
+  BE.to = mk_to_k256_cm;
+  BE.lmul = point_add;
+  BE.lsqr = point_double;
+}
+
+//////////////////////////////////////////////////////
+
+inline_for_extraction noextract
+val make_point_at_inf: p:point -> Stack unit
+  (requires fun h -> live h p)
+  (ensures  fun h0 _ h1 -> modifies (loc p) h0 h1 /\
+    point_inv h1 p /\
+    S.to_aff_point (point_as_nat3_proj h1 p) == S.aff_point_at_inf)
+
+let make_point_at_inf p =
+  let px, py, pz = getx p, gety p, getz p in
+  set_zero px;
+  set_one py;
+  set_zero pz;
+  S.to_aff_point_at_infinity_lemma ()
+
+
+inline_for_extraction noextract
+val make_g: g:point -> Stack unit
+  (requires fun h -> live h g)
+  (ensures  fun h0 _ h1 -> modifies (loc g) h0 h1 /\
+    point_inv h1 g /\
+    point_as_nat3_proj h1 g == S.g)
+
+let make_g g =
+  let gx, gy, gz = getx g, gety g, getz g in
+  make_u64_4 gx
+    (u64 0x59f2815b16f81798)
+    (u64 0x029bfcdb2dce28d9)
+    (u64 0x55a06295ce870b07)
+    (u64 0x79be667ef9dcbbac);
+
+  assert_norm (S.g_x == as_nat4
+    (u64 0x59f2815b16f81798,
+     u64 0x029bfcdb2dce28d9,
+     u64 0x55a06295ce870b07,
+     u64 0x79be667ef9dcbbac));
+
+  make_u64_4 gy
+    (u64 0x9c47d08ffb10d4b8)
+    (u64 0xfd17b448a6855419)
+    (u64 0x5da4fbfc0e1108a8)
+    (u64 0x483ada7726a3c465);
+
+  assert_norm (S.g_y == as_nat4
+    (u64 0x9c47d08ffb10d4b8,
+     u64 0xfd17b448a6855419,
+     u64 0x5da4fbfc0e1108a8,
+     u64 0x483ada7726a3c465));
+
+  set_one gz
+
+
+// TODO: fix extraction for bn_from_bytes_le/be
+val point_mul: out:point -> scalar:lbuffer uint8 32ul -> q:point -> Stack unit
+  (requires fun h ->
+    live h out /\ live h scalar /\ live h q /\
+    disjoint out q /\ disjoint out scalar /\ disjoint q scalar /\
+    point_inv h q)
+  (ensures  fun h0 _ h1 -> modifies (loc out) h0 h1 /\
+    point_inv h1 out /\
+    S.to_aff_point (point_as_nat3_proj h1 out) ==
+    S.to_aff_point (S.point_mul (as_seq h0 scalar) (point_as_nat3_proj h0 q)))
+
+[@CInline]
+let point_mul out scalar q =
+  let h0 = ST.get () in
+  push_frame ();
+  let bscalar = create 4ul (u64 0) in
+  BC.bn_from_bytes_be 32ul scalar bscalar;
+  SC.bn_from_bytes_be_lemma #U64 32 (as_seq h0 scalar);
+
+  make_point_at_inf out;
+  BE.lexp_fw_consttime 12ul 0ul mk_k256_concrete_ops (null uint64) q 4ul 256ul bscalar out 4ul;
+  pop_frame ()
+
+
+val point_mul_double_vartime:
+    out:point
+  -> scalar1:lbuffer uint8 32ul
+  -> q1:point
+  -> scalar2:lbuffer uint8 32ul
+  -> q2:point ->
+  Stack unit
+  (requires fun h ->
+    live h out /\ live h scalar1 /\ live h q1 /\ live h scalar2 /\ live h q2 /\
+    disjoint q1 out /\ disjoint q2 out /\ disjoint q1 q2 /\
+    point_inv h q1 /\ point_inv h q2)
+  (ensures fun h0 _ h1 -> modifies (loc out) h0 h1 /\
+    point_inv h1 out /\
+    S.to_aff_point (point_as_nat3_proj h1 out) ==
+    S.to_aff_point (S.point_mul_double
+      (as_seq h0 scalar1) (point_as_nat3_proj h0 q1)
+      (as_seq h0 scalar2) (point_as_nat3_proj h0 q2)))
+
+[@CInline]
+let point_mul_double_vartime out scalar1 q1 scalar2 q2 =
+  let h0 = ST.get () in
+  push_frame ();
+  let bscalar1 = create 4ul (u64 0) in
+  BC.bn_from_bytes_be 32ul scalar1 bscalar1;
+  SC.bn_from_bytes_be_lemma #U64 32 (as_seq h0 scalar1);
+
+  let bscalar2 = create 4ul (u64 0) in
+  BC.bn_from_bytes_be 32ul scalar2 bscalar2;
+  SC.bn_from_bytes_be_lemma #U64 32 (as_seq h0 scalar2);
+
+  make_point_at_inf out;
+  ME.lexp_double_fw_vartime 12ul 0ul mk_k256_concrete_ops (null uint64) q1 4ul 256ul bscalar1 q2 bscalar2 out 4ul;
+  pop_frame ()
+
+
+val point_mul_g: out:point -> scalar:lbuffer uint8 32ul -> Stack unit
+  (requires fun h ->
+    live h scalar /\ live h out /\ disjoint out scalar)
+  (ensures  fun h0 _ h1 -> modifies (loc out) h0 h1 /\
+    point_inv h1 out /\
+    S.to_aff_point (point_as_nat3_proj h1 out) ==
+    S.to_aff_point (S.point_mul_g (as_seq h0 scalar)))
+
+[@CInline]
+let point_mul_g out scalar =
+  push_frame ();
+  let g = create 12ul (u64 0) in
+  make_g g;
+  point_mul out scalar g;
+  pop_frame ()
+
+
+val point_mul_g_double_vartime:
+    out:point
+  -> scalar1:lbuffer uint8 32ul
+  -> scalar2:lbuffer uint8 32ul
+  -> q2:point ->
+  Stack unit
+  (requires fun h ->
+    live h out /\ live h scalar1 /\ live h scalar2 /\ live h q2 /\
+    disjoint q2 out /\
+    point_inv h q2)
+  (ensures fun h0 _ h1 -> modifies (loc out) h0 h1 /\
+    point_inv h1 out /\
+    S.to_aff_point (point_as_nat3_proj h1 out) ==
+    S.to_aff_point (S.point_mul_double_g
+      (as_seq h0 scalar1) (as_seq h0 scalar2) (point_as_nat3_proj h0 q2)))
+
+[@CInline]
+let point_mul_g_double_vartime out scalar1 scalar2 q2 =
+  push_frame ();
+  let g = create 12ul (u64 0) in
+  make_g g;
+  point_mul_double_vartime out scalar1 g scalar2 q2;
+  pop_frame ()
